messageInvariantPrototypes/clientServer/messageInvariants.dfy
@@ -8,46 +8,53 @@ import opened DistributedSystem
 import opened Obligations
 
 // certified self inductive, modulo requires
-predicate RequestsValidSource(c: Constants, v: Variables) 
+// Every request message in the network has a proper source
+predicate RequestMsgsValidSource(c: Constants, v: Variables) 
   requires v.WF(c)
 {
-  forall req | req in v.network.sentMsgs && req.Request?
-  :: c.ValidClientIdx(req.clientId)
+  forall req | req in v.network.sentMsgs && req.RequestMsg?
+  :: c.ValidClientIdx(req.r.clientId)
 }
 
 // certified self inductive, modulo requires
-predicate ResponseCorrespondToRequest(c: Constants, v: Variables)
+// Every request message in the network comes from the source's request set
+// Property of Send
+predicate RequestMsgsValid(c: Constants, v: Variables)
   requires v.WF(c)
+  requires RequestMsgsValidSource(c, v)
 {
-  forall resp | resp in v.network.sentMsgs && resp.Response?
-  :: Request(resp.clientId, resp.reqId) in v.network.sentMsgs
+  forall req | req in v.network.sentMsgs && req.RequestMsg?
+  :: req.r.reqId in v.hosts[req.r.clientId].client.requests
 }
 
 // certified self inductive, modulo requires
-predicate RequestMessagesValid(c: Constants, v: Variables)
+// Every request message in the network comes from the source's request set
+// Property of Receive
+predicate ServerCurrentRequestValid(c: Constants, v: Variables)
   requires v.WF(c)
-  requires RequestsValidSource(c, v)
 {
-  forall req | req in v.network.sentMsgs && req.Request?
-  :: req.reqId in v.hosts[req.clientId].client.requests
+  forall idx:nat | c.ValidServerIdx(idx) && v.hosts[idx].server.currentRequest.Some?
+  :: RequestMsg(v.hosts[idx].server.currentRequest.value) in v.network.sentMsgs
 }
 
 // certified self inductive, modulo requires
-predicate ReceivedResponsesValid(c: Constants, v: Variables)
+// Every client's collected responses came from the network.
+// Property of Receive
+predicate ClientResponsesValid(c: Constants, v: Variables)
   requires v.WF(c)
 {
   forall idx:nat, respId | c.ValidClientIdx(idx) && respId in v.hosts[idx].client.responses
-  :: Response(idx, respId) in v.network.sentMsgs
+  :: ResponseMsg(Req(idx, respId)) in v.network.sentMsgs
 }
 
 
 predicate MessageInv(c: Constants, v: Variables) 
 {
   && v.WF(c)
-  && RequestsValidSource(c, v)
-  && ResponseCorrespondToRequest(c, v)
-  && RequestMessagesValid(c, v)
-  && ReceivedResponsesValid(c, v)
+  && RequestMsgsValidSource(c, v)
+  && RequestMsgsValid(c, v)
+  && ServerCurrentRequestValid(c, v)
+  && ClientResponsesValid(c, v)
 }
 
 lemma InitImpliesMessageInv(c: Constants, v: Variables)
