messageInvariantPrototypes/clientServer/readme.md
@@ -1,3 +1,5 @@
 This is the "client_server_ae" protocol from [DuoAI](https://github.com/VeriGu/DuoAI/tree/master/protocols) (OSDI'22). 
 
 Multiple clients can send requests to a server. The server processes each request and returns a response to the respective client. The server may process the requests out-of-order.
+
+However, compared to "client_server_ae", server receives requests and send response in separate steps, rather than one atomic step. This is to add some degree of complexity to the protocol and proof.
